src/All.ec
@@ -1,0 +1,20 @@
+require Constants.
+require EllipticCurve.
+require ExtractedTests.
+require Field.
+require Memory.
+require PurePrimops.
+require UInt256.
+require Utils.
+require Verifier.
+require VerifierConsts.
+require YulPrimops.
+require YulTests.
+(* specs *)
+require EvaluateLagrangePolyOutOfDomain.
+require LookupQuotientContribution.
+require Modexp.
+require PermutationQuotientContribution.
+require PointNegate.
+require RevertWithMessage.
+require VerifyQuotientEvaluation.
